lib/pulse/lib/Pulse.Lib.WhileLoop.fsti
@@ -12,3 +12,11 @@ fn while_loop
   (body : stt unit (inv true) (fun _ -> exists* x. inv x))
   requires exists* x. inv x
   ensures inv false
+
+fn nuwhile_loop
+  (inv : slprop)
+  (cpost : bool -> slprop)
+  (cond : stt bool inv (fun b -> cpost b))
+  (body : stt unit (cpost true) (fun _ -> inv))
+  requires inv
+  ensures  cpost false
