src/checker/Pulse.Checker.NuWhile.fst
@@ -1,0 +1,305 @@
+(*
+   Copyright 2023 Microsoft Research
+
+   Licensed under the Apache License, Version 2.0 (the "License");
+   you may not use this file except in compliance with the License.
+   You may obtain a copy of the License at
+
+       http://www.apache.org/licenses/LICENSE-2.0
+
+   Unless required by applicable law or agreed to in writing, software
+   distributed under the License is distributed on an "AS IS" BASIS,
+   WITHOUT WARRANTIES OR CONDITIONS OF ANY KIND, either express or implied.
+   See the License for the specific language governing permissions and
+   limitations under the License.
+*)
+
+module Pulse.Checker.NuWhile
+
+open Pulse
+open Pulse.Syntax
+open Pulse.Typing
+open Pulse.Checker.Pure
+open Pulse.Checker.Base
+open Pulse.Checker.Prover
+open Pulse.Show
+open Pulse.PP
+open Pulse.Reflection.Util { mk_abs }
+
+module T = FStar.Tactics.V2
+module RU = Pulse.RuntimeUtils
+module Metatheory = Pulse.Typing.Metatheory
+
+let debug () : T.Tac bool =
+  RU.debug_at_level (T.top_env ()) "nuwhile"
+
+let unit_is_type0 (g:env) : tot_typing g (`unit) (tm_type T.Uv_Zero) = RU.magic ()
+
+#set-options "--z3rlimit 20"
+
+let rec drop (n:nat) (xs : list 'a) : T.Tac (list 'a) =
+  match n, xs with
+  | 0, _ -> xs
+  | _, [] -> []
+  | _, x::xs' -> drop (n-1) xs'
+
+let rec take (n:nat) (xs : list 'a) : T.Tac (list 'a) =
+  match n, xs with
+  | 0, _ -> []
+  | _, [] -> []
+  | _, x::xs' ->
+    let xs'' = take (n-1) xs' in
+    x::xs''
+
+let close1
+  (x : var)
+  (nm : ppname)
+  (xt : typ)
+  (ctxt : term)
+  : T.Tac term
+= 
+  if not (x `Set.mem` freevars ctxt) then
+    (* Easy case, it doesn't appear so just ignore it. (TODO: consider
+    refinements...) *)
+    ctxt
+  else (
+    // T.print (Printf.sprintf "closing %s for term %s" (show #int x) (show ctxt));
+    let b : binder = {binder_ppname = nm; binder_ty = xt; binder_attrs = Sealed.seal []} in
+    (* u0 is wrong *)
+    let ctxt = Syntax.Naming.close_term ctxt x in
+    let res = tm_exists_sl u0 b ctxt in
+    // T.print (Printf.sprintf "closing %s for term %s done, res = %s" (show #int x) (show ctxt) (show res));
+    res
+  )
+
+let close1_wt
+  (#g:env)
+  (x : var{~ (x `Set.mem` dom g)})
+  (nm : ppname)
+  (xt : typ)
+  (ctxt : term)
+  (ctxt_typing : tot_typing (push_binding g x nm xt) ctxt tm_slprop)
+  : T.Tac (ctxt':term & tot_typing g ctxt' tm_slprop)
+= admit()
+
+let close_into
+  (#g2:env)
+  (ctxt : term)
+  (ctxt_typing : tot_typing g2 ctxt tm_slprop)
+  (g1 : env{g2 `env_extends` g1})
+  : T.Tac (ctxt':term & tot_typing g1 ctxt' tm_slprop)
+=
+  let extra_vars = take (List.length (bindings g2) - List.length (bindings g1)) (bindings g2) in
+  // assert (g2 == push_env g1 extra_vars);
+  let ctxt' =
+    T.fold_right (fun (v,t) ctxt' ->
+      (* huge hack for the proof, this will need an aux lte rec instead of a fold. *)
+      let ctxt'' = close1 v ppname_default t ctxt' in
+      ctxt''
+    ) extra_vars ctxt
+  in
+  let d : tot_typing g1 ctxt' tm_slprop = RU.magic () in
+  (| ctxt', d |)
+
+
+#set-options "--z3rlimit 40"
+
+let check
+  (g:env)
+  (pre:term)
+  (pre_typing:tot_typing g pre tm_slprop)
+  (post_hint:post_hint_opt g)
+  (res_ppname:ppname)
+  (t:st_term{Tm_NuWhile? t.term})
+  (check:check_t)
+  : T.Tac (checker_result_t g pre post_hint) =
+  admit();
+  let g = push_context "nuwhile loop" t.range g in
+  let Tm_NuWhile { condition; body; invariant; } = t.term in
+  let (| invariant, invariant_typing |) = check_slprop g invariant in
+
+  let invariant_typing_orig : tot_typing g invariant tm_slprop = invariant_typing in
+
+  (* First thing we do is prove the invariant. Essentially
+  this is very similar to having `assert invariant` at this point.
+  After doing so, we split the context into invariant ** frame.
+  We keep the frame--- it is passed through to the checks for
+  cond and body. *)
+
+  let no_uvs = mk_env (fstar_env g) in
+
+  let (| g1, nts, _, frame, k_frame |) =
+    Prover.prove false pre_typing no_uvs invariant_typing
+  in
+
+  Tactics.BreakVC.break_vc ();
+
+  let invariant_typing : tot_typing g1 invariant tm_slprop =
+    Typing.Metatheory.tot_typing_weakening_standard g invariant_typing g1
+  in
+
+  let frame_typing : tot_typing g1 frame tm_slprop =
+    (* Prover should ensure this... *)
+    RU.magic ()
+  in
+  let frame_typing_orig : tot_typing g frame tm_slprop =
+    (* I think? *)
+    RU.magic ()
+  in
+
+  if debug () then
+    info_doc g (Some t.range) [
+      text "Proved invariant";
+      text "Frame:" ^/^ pp frame;
+    ];
+
+  (* We proved the invariant and got a frame. We now check
+  the condition in the *full* context of inv ** frame. This
+  is so we don't have to specify random fixed resources in
+  the invariant. *)
+
+  let cond_ppname = mk_ppname_no_range "cond" in
+  let (| cond_x, __g2, _booltyping, (| ctxt_after_cond, ctxt_after_cond_typing |), k_cond |) =
+    check
+      (push_context "check_while_condition" condition.range g1)
+      (tm_star invariant frame)
+      (star_typing invariant_typing frame_typing)
+      None
+      cond_ppname
+      condition
+  in
+
+  let flipped_g2 =
+    let extra_vars = take (List.length (bindings __g2) - List.length (bindings g1)) (bindings __g2) in
+    T.guard (Cons? extra_vars);
+    (* note: snoc list *)
+    let last :: init = extra_vars in
+    assume (~(Set.mem (fst last) (dom g1)));
+    let g = push_binding g1 (fst last) ppname_default (snd last) in
+    let g = T.fold_right (fun b g ->
+      let x, t = b in
+      assume (~(Set.mem x (dom g)));
+      push_binding g x ppname_default t
+    ) init g
+    in
+    g
+  in
+  let g2 = flipped_g2 in
+  let ctxt_after_cond_typing : tot_typing g2 ctxt_after_cond tm_slprop =
+    RU.magic ()
+  in
+  assume (g2 `env_extends` g1);
+
+  if debug () then
+    info_doc g (Some t.range) [
+      text "After condition:" ^/^ pp ctxt_after_cond;
+      text "g2:" ^/^ pp g2;
+    ];
+
+  let cpost =
+    let b : T.binder = {
+      uniq = cond_x;
+      ppname = cond_ppname.name;
+      sort = (`bool);
+      qual = T.Q_Explicit;
+      attrs = [];
+    } in
+    assume (~(Set.mem cond_x (dom g)));
+    let g1x = push_binding g cond_x ppname_default (`bool) in
+    assume (env_extends g2 g1x);
+    let (| ctxt_after_cond, _|) = close_into #g2 ctxt_after_cond ctxt_after_cond_typing g1x in
+    if debug () then
+      info_doc g (Some t.range) [
+        text "GG ctxt_after_cond:" ^/^ pp ctxt_after_cond;
+        text "GG cond_x = " ^/^ pp #int cond_x;
+      ];
+    T.mk_abs [b] ctxt_after_cond
+  in
+  if debug () then
+    info_doc g (Some t.range) [
+      text "Proved condition";
+      text "Condition:" ^/^ pp condition;
+      text "After condition:" ^/^ pp ctxt_after_cond;
+      text "cpost:" ^/^ pp cpost;
+    ];
+  let cpost_typing : tot_typing g1 cpost (mk_abs (`bool) T.Q_Explicit tm_slprop) = RU.magic () in
+    // Metatheory.tot_typing_weakening_standard g1 (star_typing invariant_typing frame_typing) g2
+
+  (* Check the body, in the context after checking the condition,
+     but also adding a pure fact that the condition is true. *)
+    assert (g2 `env_extends` g1);
+    let cond_x_tm = tm_var {nm_index=cond_x;nm_ppname=cond_ppname} in
+    let ctxt_after_cond_true =
+      tm_star ctxt_after_cond (tm_pure (mk_eq2 T.Uv_Zero (`bool) cond_x_tm (`true)))
+    in
+    let ctxt_after_cond_true_typing : tot_typing g2 ctxt_after_cond_true tm_slprop =
+      star_typing #_ #ctxt_after_cond #(tm_pure (mk_eq2 T.Uv_Zero (`bool) cond_x_tm (`true)))
+        ctxt_after_cond_typing (RU.magic ())
+    in
+    let post = tm_star invariant frame in
+    let body_st_comp : st_comp =
+      {
+        pre = tm_emp; // irrelevant
+        post = post;
+        res = (`unit);
+        u = T.Uv_Zero
+      }
+    in
+    let body_comp : comp = C_ST body_st_comp in
+    let x = fresh g2 in
+    assume (~(x `Set.mem` freevars post)); // prove
+    assume (open_term post x == post); // prove
+    let g2x = push_binding g2 x ppname_default (`unit) in
+    assert (g2 `env_extends` g1);
+    assume (g2x `env_extends` g1); // trivial?
+    let body_comp_typing : comp_typing_u g2 body_comp =
+      CT_ST g2 body_st_comp <| STC g2 body_st_comp x
+                     (unit_is_type0 _)
+                     emp_typing
+                     (Metatheory.tot_typing_weakening_standard
+                       g1
+                       (star_typing invariant_typing frame_typing)
+                       g2x)
+    in
+  let body_hint : post_hint_for_env g2 = post_hint_from_comp_typing body_comp_typing in
+  let after_body =
+    check
+      (push_context "check_while_body" body.range g2)
+      ctxt_after_cond_true
+      ctxt_after_cond_true_typing
+      (Some body_hint)
+      res_ppname
+      body
+  in
+  let (| body', body'_comp, body'_typing |) =
+    apply_checker_result_k after_body (mk_ppname_no_range "_nuwhile_b")
+  in
+  let (| body', body'_comp, body'_typing |) =
+    let pak () : Typing.Combinators.st_typing_in_ctxt __g2 ctxt_after_cond_true (Some body_hint) =
+      admit();
+      (| body', body'_comp, body'_typing |)
+    in
+    admit();
+    k_cond (Some body_hint) (pak ())
+  in
+  admit();
+
+  info_doc g (Some t.range) [
+    text "NUWHILE After body:" ^/^ pp body';
+  ];
+
+  let d : st_typing g1 _ _ =
+    T_NuWhile
+    g1
+    (tm_star invariant frame)
+    condition
+    cpost body'
+    (star_typing invariant_typing frame_typing)
+    cpost_typing
+  in
+  assume (comp_pre (comp_nuwhile (tm_star invariant frame) cpost) == pre);
+  assume (comp_post_matches_hint (comp_nuwhile (tm_star invariant frame) cpost) post_hint);
+  let (| t, c, d |) = k_frame post_hint (| _, _, d |) in
+  prove_post_hint
+    (try_frame_pre false pre_typing (match_comp_res_with_post_hint d post_hint) res_ppname)
+    post_hint t.range
