src/checker/Pulse.Checker.fst
@@ -39,6 +39,7 @@ module Match = Pulse.Checker.Match
 module WithLocal = Pulse.Checker.WithLocal
 module WithLocalArray = Pulse.Checker.WithLocalArray
 module While = Pulse.Checker.While
+module NuWhile = Pulse.Checker.NuWhile
 module STApp = Pulse.Checker.STApp
 module Exists = Pulse.Checker.Exists
 module Par = Pulse.Checker.Par
@@ -302,6 +303,9 @@ let rec check
         )
         | Tm_While _ ->
           While.check g pre pre_typing post_hint res_ppname t check
+
+        | Tm_NuWhile _ ->
+          NuWhile.check g pre pre_typing post_hint res_ppname t check
 
         | Tm_Match {sc;returns_=post_match;brs} ->
           // TODO : dedup
