test/nolib/NuWhile.fst
@@ -1,0 +1,118 @@
+module NuWhile
+
+#lang-pulse
+open Pulse.Nolib
+
+assume val p : int -> slprop
+
+fn chk (x : int)
+  requires p x
+  returns  bool
+  ensures  p x
+{ false }
+
+fn use (x : int)
+  requires p x
+  ensures  p x
+{ () }
+
+ghost
+fn use_ghost (x : int)
+  requires p x
+  ensures  p x
+{ () }
+
+ghost
+fn use_ghost_incr (x : int)
+  requires p x
+  ensures  p (x+1)
+{ admit() }
+
+[@@expect_failure] // kinda silly that this fails
+fn nohint()
+{
+  { (); (); };
+  ()
+}
+
+fn test0 ()
+  requires p 1 ** p 2 ** p 3
+  ensures  p 1 ** p 2 ** p 3
+{
+  nuwhile (chk 2)
+    (* Invariant is inferred to be the full context: p 1 ** p 2 ** p 3 *)
+    (* We can also specify any of them here (only once, of course, they are
+    combined with ** ), that does not change much. *)
+    invariant p 1
+    invariant p 2
+  { use 3; use 2; };
+  ();
+  (* all resources are still there *)
+  use 1;
+  use 2;
+  use 3;
+}
+
+fn test1 ()
+  requires exists* x. p x
+  ensures  exists* x. p x
+{
+  nuwhile (true)
+    (* The invariant (= ctxt) here is inferred to be p x0, with x0 having been
+    eliminated into the environment. *)
+  { use_ghost _; };
+  ();
+  use_ghost _;
+}
+
+[@@expect_failure]
+fn test2 ()
+  requires exists* x. p x
+  ensures exists* x. p x
+{
+  nuwhile (true)
+    (* Same as above, but that invariant does not work as we are
+    changing x every iteration. *)
+  { use_ghost_incr _; };
+  ();
+}
+
+assume val q : slprop
+
+fn use_q ()
+  requires q
+  ensures  q
+{ () }
+
+fn test3 ()
+  requires q ** (exists* x. p x)
+  ensures  q ** (exists* x. p x)
+{
+  // with x. assert (p x);
+  nuwhile (false)
+    (* Specifying a weaker invariant works. *)
+    invariant exists* x. p x
+  { 
+    assert q;
+    use_q ();
+    use_ghost_incr _;
+  };
+  use_ghost _;
+  assert q;
+  // chk _;
+  use_ghost _;
+  ()
+}
+
+
+fn true_cond ()
+  returns b : bool
+  ensures pure (b == true)
+{ true }
+
+fn test_inf_loop ()
+{
+  nuwhile (true_cond ())
+  { () };
+  assert (pure False);
+}
